Rename heapVars to domA

Launchbury/DistinctVars.thy
@@ -2,58 +2,53 @@ theory DistinctVars
 imports Main "~~/src/HOL/Library/AList"
 begin
 
+text {* We want to have @{text delete} and @{text update} back in the namespace. *}
+
 abbreviation delete where "delete \<equiv> AList.delete"
 abbreviation update where "update \<equiv> AList.update"
 
-lemma delete_append[simp]: "delete x (l1 @ l2) = delete x l1 @ delete x l2"
-  unfolding AList.delete_eq by simp
+subsubsection {* The domain of an associative list *}
 
-subsubsection {* The domain of a associative list *}
+definition domA
+  where "domA h = fst ` set h"
 
-definition heapVars
-  where "heapVars h = fst ` set h"
+lemma domA_append[simp]:"domA (a @ b) = domA a \<union> domA b"
+  and [simp]:"domA ((v,e) # h) = insert v (domA h)"
+  and [simp]:"domA (p # h) = insert (fst p) (domA h)"
+  and [simp]:"domA [] = {}"
+  by (auto simp add: domA_def)
 
-lemma heapVarsAppend[simp]:"heapVars (a @ b) = heapVars a \<union> heapVars b"
-  and [simp]:"heapVars ((v,e) # h) = insert v (heapVars h)"
-  and [simp]:"heapVars (p # h) = insert (fst p) (heapVars h)"
-  and [simp]:"heapVars [] = {}"
-  by (auto simp add: heapVars_def)
-
-lemma heapVars_from_set:
-  "(x, e) \<in> set h \<Longrightarrow> x \<in> heapVars h"
+lemma domA_from_set:
+  "(x, e) \<in> set h \<Longrightarrow> x \<in> domA h"
 by (induct h, auto)
 
-lemma finite_heapVars[simp]:
-  "finite (heapVars \<Gamma>)"
-  by (auto simp add: heapVars_def)
+lemma finite_domA[simp]:
+  "finite (domA \<Gamma>)"
+  by (auto simp add: domA_def)
 
-lemma delete_no_there:
-  "x \<notin> heapVars \<Gamma> \<Longrightarrow> delete x \<Gamma> = \<Gamma>"
+lemma domA_delete[simp]:
+  "domA (delete x \<Gamma>) = domA \<Gamma> - {x}"
   by (induct \<Gamma>, auto)
 
-lemma heapVars_delete[simp]:
-  "heapVars (delete x \<Gamma>) = heapVars \<Gamma> - {x}"
-  by (induct \<Gamma>, auto)
+lemma dom_map_of_conv_domA:
+  "dom (map_of \<Gamma>) = domA \<Gamma>"
+  by (induct \<Gamma>) (auto simp add: dom_if)
 
+subsubsection {* Other lemmas about associative lists *}
 
-lemma dom_map_of_conv_heapVars:
-  "dom (map_of xys) = heapVars xys"
-  by (induct xys) (auto simp add: dom_if)
-
+lemma delete_append[simp]: "delete x (l1 @ l2) = delete x l1 @ delete x l2"
+  unfolding AList.delete_eq by simp
 
 lemma map_of_delete_insert:
   assumes "map_of \<Gamma> x = Some e"
   shows "map_of ((x,e) # delete x \<Gamma>) = map_of \<Gamma>"
   using assms by (induct \<Gamma>) (auto split:prod.split)
 
-lemma map_add_heapVars[simp]: 
-  "x \<in> heapVars \<Gamma> \<Longrightarrow> (map_of \<Delta> ++ map_of \<Gamma>) x = map_of \<Gamma> x"
-  "x \<notin> heapVars \<Gamma> \<Longrightarrow> (map_of \<Delta> ++ map_of \<Gamma>) x = map_of \<Delta> x"
-    apply (metis dom_map_of_conv_heapVars map_add_dom_app_simps(1))
-    apply (metis dom_map_of_conv_heapVars map_add_dom_app_simps(3))
+lemma map_add_domA[simp]: 
+  "x \<in> domA \<Gamma> \<Longrightarrow> (map_of \<Delta> ++ map_of \<Gamma>) x = map_of \<Gamma> x"
+  "x \<notin> domA \<Gamma> \<Longrightarrow> (map_of \<Delta> ++ map_of \<Gamma>) x = map_of \<Delta> x"
+    apply (metis dom_map_of_conv_domA map_add_dom_app_simps(1))
+    apply (metis dom_map_of_conv_domA map_add_dom_app_simps(3))
     done
 
-lemma the_map_of_snd:
-  "x\<in> heapVars \<Gamma> \<Longrightarrow> the (map_of \<Gamma> x) \<in> snd ` set \<Gamma>"
-by (induct \<Gamma>, auto)
 end
