Launchbury/CorrectnessOriginal.thy
@@ -6,12 +6,12 @@ text {*
 This is the main correctness theorem, Theorem 2 from \cite{launchbury}.
 *}
 
-(* Another possible invariant seems to be: "fdom \<rho> - heapVars \<Gamma> \<subseteq> set L" *)
+(* Another possible invariant seems to be: "fdom \<rho> - domA \<Gamma> \<subseteq> set L" *)
 
 theorem correctness:
   assumes "\<Gamma> : e \<Down>\<^bsub>L\<^esub> \<Delta> : z"
-  and     "fv (\<Gamma>, e) - heapVars \<Gamma> \<subseteq> set L"
-  shows   "\<lbrakk>e\<rbrakk>\<^bsub>\<lbrace>\<Gamma>\<rbrace>\<rho>\<^esub> = \<lbrakk>z\<rbrakk>\<^bsub>\<lbrace>\<Delta>\<rbrace>\<rho>\<^esub>" and "(\<lbrace>\<Gamma>\<rbrace>\<rho>) f|` heapVars \<Gamma> = (\<lbrace>\<Delta>\<rbrace>\<rho>) f|` heapVars \<Gamma>"
+  and     "fv (\<Gamma>, e) - domA \<Gamma> \<subseteq> set L"
+  shows   "\<lbrakk>e\<rbrakk>\<^bsub>\<lbrace>\<Gamma>\<rbrace>\<rho>\<^esub> = \<lbrakk>z\<rbrakk>\<^bsub>\<lbrace>\<Delta>\<rbrace>\<rho>\<^esub>" and "(\<lbrace>\<Gamma>\<rbrace>\<rho>) f|` domA \<Gamma> = (\<lbrace>\<Delta>\<rbrace>\<rho>) f|` domA \<Gamma>"
   using assms
 proof(nominal_induct arbitrary: \<rho> rule:reds.strong_induct)
 case Lambda
@@ -21,28 +21,28 @@ next
 case (Application y \<Gamma> e x L \<Delta> \<Theta> z e')
   hence "y \<noteq> x" by (simp_all add: fresh_at_base)
 
-  have Gamma_subset: "heapVars \<Gamma> \<subseteq> heapVars \<Delta>"
+  have Gamma_subset: "domA \<Gamma> \<subseteq> domA \<Delta>"
     by (rule reds_doesnt_forget[OF Application.hyps(8)])
 
   case 1
-  hence prem1: "fv (\<Gamma>, e) - heapVars \<Gamma> \<subseteq> set (x#L)" by auto
+  hence prem1: "fv (\<Gamma>, e) - domA \<Gamma> \<subseteq> set (x#L)" by auto
 
-  from 1 Gamma_subset have *: "x \<in> set L \<or> x \<in> heapVars \<Delta>" by auto
+  from 1 Gamma_subset have *: "x \<in> set L \<or> x \<in> domA \<Delta>" by auto
 
-  have "fv (\<Delta>, e'[y::=x]) - heapVars \<Delta> \<subseteq> (fv (\<Delta>, Lam [y]. e') - heapVars \<Delta>) \<union> {x}"
+  have "fv (\<Delta>, e'[y::=x]) - domA \<Delta> \<subseteq> (fv (\<Delta>, Lam [y]. e') - domA \<Delta>) \<union> {x}"
     by (auto dest!: set_mp[OF fv_subst_subset])
-  also have "\<dots> \<subseteq> (fv (\<Gamma>, e) - heapVars \<Gamma>) \<union> {x}"
+  also have "\<dots> \<subseteq> (fv (\<Gamma>, e) - domA \<Gamma>) \<union> {x}"
     using new_free_vars_on_heap[OF Application.hyps(8)] by auto
   also have "\<dots> \<subseteq> set L \<union> {x}" using prem1 by auto
-  finally have "fv (\<Delta>, e'[y::=x]) - heapVars \<Delta> \<subseteq> set L \<union> {x}". 
+  finally have "fv (\<Delta>, e'[y::=x]) - domA \<Delta> \<subseteq> set L \<union> {x}". 
   with *
-  have prem2: "fv (\<Delta>, e'[y::=x]) - heapVars \<Delta> \<subseteq> set L" by auto
+  have prem2: "fv (\<Delta>, e'[y::=x]) - domA \<Delta> \<subseteq> set L" by auto
   
   have *: "(\<lbrace>\<Gamma>\<rbrace>\<rho>) x = (\<lbrace>\<Delta>\<rbrace>\<rho>) x"
-  proof(cases "x \<in> heapVars \<Gamma>")
+  proof(cases "x \<in> domA \<Gamma>")
     case True
     from Application.hyps(10)[OF prem1, where \<rho> = \<rho>]
-    have "((\<lbrace>\<Gamma>\<rbrace>\<rho>) f|` heapVars \<Gamma>) x  = ((\<lbrace>\<Delta>\<rbrace>\<rho>) f|` heapVars \<Gamma>) x" by simp
+    have "((\<lbrace>\<Gamma>\<rbrace>\<rho>) f|` domA \<Gamma>) x  = ((\<lbrace>\<Delta>\<rbrace>\<rho>) f|` domA \<Gamma>) x" by simp
     with True show ?thesis by simp
   next
     case False 
@@ -67,42 +67,42 @@ case (Application y \<Gamma> e x L \<Delta> \<Theta> z e')
   finally
   show ?case.
   
-  show "(\<lbrace>\<Gamma>\<rbrace>\<rho>) f|` heapVars \<Gamma> = (\<lbrace>\<Theta>\<rbrace>\<rho>) f|` heapVars \<Gamma>"
+  show "(\<lbrace>\<Gamma>\<rbrace>\<rho>) f|` domA \<Gamma> = (\<lbrace>\<Theta>\<rbrace>\<rho>) f|` domA \<Gamma>"
     using Application.hyps(10)[OF prem1]
           fmap_restr_eq_subset[OF Gamma_subset Application.hyps(13)[OF prem2]]
     by (rule trans)
 next
 case (Variable \<Gamma> x e L \<Delta> z)
-  hence [simp]:"x \<in> heapVars \<Gamma>" by (metis heapVars_from_set map_of_is_SomeD)
+  hence [simp]:"x \<in> domA \<Gamma>" by (metis domA_from_set map_of_is_SomeD)
 
   case 2
-  have "x \<notin> heapVars \<Delta>"
+  have "x \<notin> domA \<Delta>"
     by (rule reds_avoids_live[OF Variable.hyps(2)], simp_all)
 
-  have subset: "heapVars (delete x \<Gamma>) \<subseteq> heapVars \<Delta>"
+  have subset: "domA (delete x \<Gamma>) \<subseteq> domA \<Delta>"
     by (rule reds_doesnt_forget[OF Variable.hyps(2)])
 
   have "fv (delete x \<Gamma>, e) \<union> {x} \<subseteq> fv (\<Gamma>, Var x)"
     by (rule fv_delete_heap[OF `map_of \<Gamma> x = Some e`])
-  hence prem: "fv (delete x \<Gamma>, e) - heapVars (delete x \<Gamma>) \<subseteq> set (x # L)" using 2 by auto
+  hence prem: "fv (delete x \<Gamma>, e) - domA (delete x \<Gamma>) \<subseteq> set (x # L)" using 2 by auto
 
-  have fv_subset: "fv (delete x \<Gamma>, e) - heapVars (delete x \<Gamma>) \<subseteq> - (heapVars \<Delta> - heapVars \<Gamma>)"
+  have fv_subset: "fv (delete x \<Gamma>, e) - domA (delete x \<Gamma>) \<subseteq> - (domA \<Delta> - domA \<Gamma>)"
     apply (rule subset_trans[OF prem])
     apply (rule subset_trans[OF reds_avoids_live'[OF Variable.hyps(2)]])
     by auto
 
-  let "?new" = "heapVars \<Delta> - heapVars \<Gamma>"
-  have "heapVars \<Gamma> \<subseteq> (-?new)" by auto
+  let "?new" = "domA \<Delta> - domA \<Gamma>"
+  have "domA \<Gamma> \<subseteq> (-?new)" by auto
 
   have "\<lbrace>\<Gamma>\<rbrace>\<rho> = \<lbrace>(x,e) # delete x \<Gamma>\<rbrace>\<rho>"
     by (rule HSem_reorder[OF map_of_delete_insert[symmetric, OF Variable(1)]])
-  also have "\<dots> = (\<mu> \<rho>'. (\<rho> f++\<^bsub>(heapVars (delete x \<Gamma>))\<^esub> (\<lbrace>delete x \<Gamma>\<rbrace>\<rho>'))( x := \<lbrakk> e \<rbrakk>\<^bsub>\<rho>'\<^esub>))"
+  also have "\<dots> = (\<mu> \<rho>'. (\<rho> f++\<^bsub>(domA (delete x \<Gamma>))\<^esub> (\<lbrace>delete x \<Gamma>\<rbrace>\<rho>'))( x := \<lbrakk> e \<rbrakk>\<^bsub>\<rho>'\<^esub>))"
     by (rule iterative_HSem, simp)
-  also have "\<dots> = (\<mu> \<rho>'. (\<rho> f++\<^bsub>(heapVars (delete x \<Gamma>))\<^esub> (\<lbrace>delete x \<Gamma>\<rbrace>\<rho>'))( x := \<lbrakk> e \<rbrakk>\<^bsub>\<lbrace>delete x \<Gamma>\<rbrace>\<rho>'\<^esub>))"
+  also have "\<dots> = (\<mu> \<rho>'. (\<rho> f++\<^bsub>(domA (delete x \<Gamma>))\<^esub> (\<lbrace>delete x \<Gamma>\<rbrace>\<rho>'))( x := \<lbrakk> e \<rbrakk>\<^bsub>\<lbrace>delete x \<Gamma>\<rbrace>\<rho>'\<^esub>))"
     by (rule iterative_HSem', simp)
   finally
   have "(\<lbrace>\<Gamma>\<rbrace>\<rho>)f|` (- ?new) = (...) f|` (- ?new)" by simp
-  also have "\<dots> = (\<mu> \<rho>'. (\<rho> f++\<^bsub>heapVars \<Delta>\<^esub> (\<lbrace>\<Delta>\<rbrace>\<rho>'))( x := \<lbrakk> z \<rbrakk>\<^bsub>\<lbrace>\<Delta>\<rbrace>\<rho>'\<^esub>)) f|` (- ?new)"
+  also have "\<dots> = (\<mu> \<rho>'. (\<rho> f++\<^bsub>domA \<Delta>\<^esub> (\<lbrace>\<Delta>\<rbrace>\<rho>'))( x := \<lbrakk> z \<rbrakk>\<^bsub>\<lbrace>\<Delta>\<rbrace>\<rho>'\<^esub>)) f|` (- ?new)"
   proof (induction rule: parallel_fix_ind[where P ="\<lambda> x y. x f|` (- ?new) = y f|` (- ?new)"])
     case 1 show ?case by simp
   next
@@ -110,21 +110,21 @@ case (Variable \<Gamma> x e L \<Delta> z)
   next
     case (3 \<sigma> \<sigma>')
     hence "\<lbrakk> e \<rbrakk>\<^bsub>\<lbrace>delete x \<Gamma>\<rbrace>\<sigma>\<^esub> = \<lbrakk> e \<rbrakk>\<^bsub>\<lbrace>delete x \<Gamma>\<rbrace>\<sigma>'\<^esub>"
-      and "(\<lbrace>delete x \<Gamma>\<rbrace>\<sigma>) f|` heapVars (delete x \<Gamma>) = (\<lbrace>delete x \<Gamma>\<rbrace>\<sigma>') f|` heapVars (delete x \<Gamma>)"
+      and "(\<lbrace>delete x \<Gamma>\<rbrace>\<sigma>) f|` domA (delete x \<Gamma>) = (\<lbrace>delete x \<Gamma>\<rbrace>\<sigma>') f|` domA (delete x \<Gamma>)"
       using fv_subset by (auto intro: ESem_fresh_cong HSem_fresh_cong  fmap_restr_eq_subset[OF _ 3])
     from trans[OF this(1) Variable(3)[OF prem]] trans[OF this(2) Variable(4)[OF prem]]
     have  "\<lbrakk> e \<rbrakk>\<^bsub>\<lbrace>delete x \<Gamma>\<rbrace>\<sigma>\<^esub> = \<lbrakk> z \<rbrakk>\<^bsub>\<lbrace>\<Delta>\<rbrace>\<sigma>'\<^esub>"
-       and "(\<lbrace>delete x \<Gamma>\<rbrace>\<sigma>) f|` heapVars (delete x \<Gamma>) = (\<lbrace>\<Delta>\<rbrace>\<sigma>') f|` heapVars (delete x \<Gamma>)".
+       and "(\<lbrace>delete x \<Gamma>\<rbrace>\<sigma>) f|` domA (delete x \<Gamma>) = (\<lbrace>\<Delta>\<rbrace>\<sigma>') f|` domA (delete x \<Gamma>)".
     thus ?case
       using subset
       by (auto intro!: ext simp add: lookup_fmap_add_eq  lookup_fmap_restr_eq dest: fmap_restr_eqD )
   qed
-  also have "\<dots> = (\<mu> \<rho>'. (\<rho> f++\<^bsub>heapVars \<Delta>\<^esub> (\<lbrace>\<Delta>\<rbrace>\<rho>'))( x := \<lbrakk> z \<rbrakk>\<^bsub>\<rho>'\<^esub>)) f|` (-?new)"
-    by (rule arg_cong[OF iterative_HSem'[symmetric], OF `x \<notin> heapVars \<Delta>`])
+  also have "\<dots> = (\<mu> \<rho>'. (\<rho> f++\<^bsub>domA \<Delta>\<^esub> (\<lbrace>\<Delta>\<rbrace>\<rho>'))( x := \<lbrakk> z \<rbrakk>\<^bsub>\<rho>'\<^esub>)) f|` (-?new)"
+    by (rule arg_cong[OF iterative_HSem'[symmetric], OF `x \<notin> domA \<Delta>`])
   also have "\<dots> = (\<lbrace>(x,z) # \<Delta>\<rbrace>\<rho>)  f|` (-?new)"
-    by (rule arg_cong[OF iterative_HSem[symmetric], OF `x \<notin> heapVars \<Delta>`])
+    by (rule arg_cong[OF iterative_HSem[symmetric], OF `x \<notin> domA \<Delta>`])
   finally
-  show le: ?case by (rule fmap_restr_eq_subset[OF `heapVars \<Gamma> \<subseteq> (-?new)`])
+  show le: ?case by (rule fmap_restr_eq_subset[OF `domA \<Gamma> \<subseteq> (-?new)`])
 
   have "\<lbrakk> Var x \<rbrakk>\<^bsub>\<lbrace>\<Gamma>\<rbrace>\<rho>\<^esub> = \<lbrakk> Var x \<rbrakk>\<^bsub>\<lbrace>(x, z) # \<Delta>\<rbrace>\<rho>\<^esub>"
     using fmap_restr_eqD[OF le, where x = x]
@@ -137,21 +137,21 @@ next
 case (Let as \<Gamma> L body \<Delta> z)
   case 1
   { fix a
-    assume a: "a \<in> heapVars (asToHeap as)"
+    assume a: "a \<in> domA (asToHeap as)"
     have "atom a \<sharp> \<Gamma>" 
-      by (rule Let(1)[unfolded fresh_star_def set_bn_to_atom_heapVars, rule_format, OF imageI[OF a]])
-    hence "a \<notin> heapVars \<Gamma>"
-      by (metis heapVars_not_fresh)
+      by (rule Let(1)[unfolded fresh_star_def set_bn_to_atom_domA, rule_format, OF imageI[OF a]])
+    hence "a \<notin> domA \<Gamma>"
+      by (metis domA_not_fresh)
   }
   note * = this
 
   
-  have "fv (asToHeap as @ \<Gamma>, body) - heapVars (asToHeap as @ \<Gamma>) \<subseteq>  fv (\<Gamma>, Let as body) - heapVars \<Gamma>"
+  have "fv (asToHeap as @ \<Gamma>, body) - domA (asToHeap as @ \<Gamma>) \<subseteq>  fv (\<Gamma>, Let as body) - domA \<Gamma>"
     by (auto dest: set_mp[OF fv_asToHeap])
-  with 1 have prem: "fv (asToHeap as @ \<Gamma>, body) - heapVars (asToHeap as @ \<Gamma>) \<subseteq> set L" by auto
+  with 1 have prem: "fv (asToHeap as @ \<Gamma>, body) - domA (asToHeap as @ \<Gamma>) \<subseteq> set L" by auto
   
-  have f1: "atom ` heapVars (asToHeap as) \<sharp>* \<Gamma>"
-    using Let(1) by (simp add: set_bn_to_atom_heapVars)
+  have f1: "atom ` domA (asToHeap as) \<sharp>* \<Gamma>"
+    using Let(1) by (simp add: set_bn_to_atom_domA)
 
   have "\<lbrakk> Let as body \<rbrakk>\<^bsub>\<lbrace>\<Gamma>\<rbrace>\<rho>\<^esub> = \<lbrakk> body \<rbrakk>\<^bsub>\<lbrace>asToHeap as\<rbrace>\<lbrace>\<Gamma>\<rbrace>\<rho>\<^esub>"
     by (simp)
@@ -162,17 +162,17 @@ case (Let as \<Gamma> L body \<Delta> z)
   finally
   show ?case.
 
-  have "(\<lbrace>\<Gamma>\<rbrace>\<rho>) f|` (heapVars \<Gamma>) = (\<lbrace>asToHeap as\<rbrace>(\<lbrace>\<Gamma>\<rbrace>\<rho>)) f|` (heapVars \<Gamma>)"
+  have "(\<lbrace>\<Gamma>\<rbrace>\<rho>) f|` (domA \<Gamma>) = (\<lbrace>asToHeap as\<rbrace>(\<lbrace>\<Gamma>\<rbrace>\<rho>)) f|` (domA \<Gamma>)"
     apply (rule ext)
-    apply (case_tac "x \<in> heapVars (asToHeap as)")
+    apply (case_tac "x \<in> domA (asToHeap as)")
     apply (auto simp add: lookup_HSem_other lookup_fmap_restr_eq *)
     done
-  also have "\<dots> = (\<lbrace>asToHeap as @ \<Gamma>\<rbrace>\<rho>) f|` (heapVars \<Gamma>)"
+  also have "\<dots> = (\<lbrace>asToHeap as @ \<Gamma>\<rbrace>\<rho>) f|` (domA \<Gamma>)"
     by (rule arg_cong[OF HSem_merge[OF f1]])
-  also have "\<dots> = (\<lbrace>\<Delta>\<rbrace>\<rho>) f|` (heapVars \<Gamma>)"
+  also have "\<dots> = (\<lbrace>\<Delta>\<rbrace>\<rho>) f|` (domA \<Gamma>)"
     by (rule fmap_restr_eq_subset[OF _ Let.hyps(5)[OF prem]]) simp
   finally
-  show "(\<lbrace>\<Gamma>\<rbrace>\<rho>) f|` heapVars \<Gamma> = (\<lbrace>\<Delta>\<rbrace>\<rho>) f|` heapVars \<Gamma>".
+  show "(\<lbrace>\<Gamma>\<rbrace>\<rho>) f|` domA \<Gamma> = (\<lbrace>\<Delta>\<rbrace>\<rho>) f|` domA \<Gamma>".
 qed
 
 end
